-

coq_v5/hott.v
@@ -2880,6 +2880,7 @@ eapply Π_type.funext; intros b₃.
 unfold hott_2_14_3.
 subst m'.
 set (m' := transport (λ X : U, X → X → X) (ua e) m : B → B → B) in *.
+simpl in m'.
 do 6 rewrite invert_compose.
 rewrite hott_2_1_4_iii.
 do 5 rewrite compose_assoc.
@@ -2887,7 +2888,15 @@ set (t := {X : Type & X → X → X}) in *.
 set (u := λ X : U, X → X → X) in *.
 set (P (xu : t) := Assoc (@pr₁ Type u xu) (@pr₂ Type u xu)) in *.
 set (p := @pair_eq Type u _ _ _ _ (ua e) (refl m')) in a'.
-subst m' a'; simpl in *.
+subst m' a'.
+do 8 rewrite <- hott_2_2_2_ii.
+do 3 rewrite hott_2_1_4_iii.
+Definition toto {A B} : ∀ (f g : A → B) (p : f == g) (x : A),
+  hap p⁻¹ x = (hap p x)⁻¹.
+Proof. destruct p; reflexivity. Defined.
+Show.
+do 2 rewrite <- toto.
+do 3 rewrite <- hott_2_2_2_ii.
 destruct e as (f, ((g, Hg), (h, Hh))); simpl.
 set (gg := existT (λ g : B → A, f ◦ g ~~ id) g Hg) in *.
 set (hh := existT (λ h0 : B → A, h0 ◦ f ~~ id) h Hh) in *.
